fix(BKS): upcasting to int in ghost is fine

AwsCryptographicMaterialProviders/dafny/AwsCryptographyKeyStore/src/HierarchicalVersionUtils.dfy
@@ -4,14 +4,17 @@ include "../../../dafny/AwsCryptographicMaterialProviders/Model/AwsCryptographyM
 include "../Model/AwsCryptographyKeyStoreTypes.dfy"
 
 module HierarchicalVersionUtils {
-
   import opened Wrappers
   import AtomicPrimitives
   import opened StandardLibrary.UInt
   import Structure
 
+  const AES_256_LENGTH: uint8 := 32
+  // BKC => Branch Key Context
+  const BKC_DIGEST_LENGTH: uint8 := 48
+  type PlainTextTuple = s: seq<uint8> | |s| == 80 witness *
+
   method ProvideCryptoClient(
-    // Crypto?: Option<AtomicPrimitives.Types.IAwsCryptographicPrimitivesClient> := None
     Crypto?: Option<AtomicPrimitives.AtomicPrimitivesClient> := None
   )
     returns (output: Result<AtomicPrimitives.AtomicPrimitivesClient, AtomicPrimitives.Types.Error>)
@@ -23,7 +26,7 @@ module HierarchicalVersionUtils {
               && fresh(output.value)
               && fresh(output.value.Modifies)
   {
-    var Crypto: AtomicPrimitives.AtomicPrimitivesClient; //AtomicPrimitives.Types.IAwsCryptographicPrimitivesClient;
+    var Crypto: AtomicPrimitives.AtomicPrimitivesClient;
     if (Crypto?.None?) {
       Crypto :- AtomicPrimitives.AtomicPrimitives();
     } else {
@@ -35,30 +38,30 @@ module HierarchicalVersionUtils {
     return Success(Crypto);
   }
 
-  // unpacks PlainTextTuple (i.e (MD_DIGEST + AES_256 key)) to return MD_DIGEST, AES_256 key
+  // unpacks PlainTextTuple (i.e (BKC_DIGEST + AES_256 key)) to return BKC_DIGEST, AES_256 key
   function UnpackPlainTextTuple (
-    plainTextTuple: seq<uint8>
+    plainTextTuple: PlainTextTuple
   ) : (Result:(seq<uint8>, seq<uint8>))
-    requires |plainTextTuple| == Structure.MD_DIGEST_LENGTH + Structure.AES_256_LENGTH
-    ensures |Result.0| == Structure.MD_DIGEST_LENGTH
-    ensures |Result.1| == Structure.AES_256_LENGTH
-    ensures Result.0 == plainTextTuple[..Structure.MD_DIGEST_LENGTH]
-    ensures Result.1 == plainTextTuple[Structure.MD_DIGEST_LENGTH..]
+    requires |plainTextTuple| == (BKC_DIGEST_LENGTH + AES_256_LENGTH) as int
+    ensures |Result.0| == BKC_DIGEST_LENGTH as int
+    ensures |Result.1| == AES_256_LENGTH as int
+    ensures Result.0 == plainTextTuple[..BKC_DIGEST_LENGTH]
+    ensures Result.1 == plainTextTuple[BKC_DIGEST_LENGTH..]
   {
-    (plainTextTuple[..Structure.MD_DIGEST_LENGTH], plainTextTuple[Structure.MD_DIGEST_LENGTH..])
+    (plainTextTuple[..BKC_DIGEST_LENGTH], plainTextTuple[BKC_DIGEST_LENGTH..])
   }
 
-  // packs mdDigest and AES 256 Key into (mdDigest + aes256Key)
+  // packs BKCDigest and AES 256 Key into (bkcDigest + aes256Key)
   function PackPlainTextTuple (
-    mdDigest: seq<uint8>, aes256Key: seq<uint8>
-  ) : (Result:(seq<uint8>))
-    requires |mdDigest| == Structure.MD_DIGEST_LENGTH
-    requires |aes256Key| == Structure.AES_256_LENGTH
-    ensures |Result| == |mdDigest| + |aes256Key|
-    ensures Result[..Structure.MD_DIGEST_LENGTH] == mdDigest
-    ensures Result[Structure.MD_DIGEST_LENGTH..] == aes256Key
-    ensures Result == mdDigest + aes256Key
+    bkcDigest: seq<uint8>, aes256Key: seq<uint8>
+  ) : (Result:(PlainTextTuple))
+    requires |bkcDigest| == BKC_DIGEST_LENGTH as int
+    requires |aes256Key| == AES_256_LENGTH as int
+    ensures |Result| as uint8 == |bkcDigest| as uint8 + |aes256Key| as uint8
+    ensures Result[..BKC_DIGEST_LENGTH] == bkcDigest
+    ensures Result[BKC_DIGEST_LENGTH..] == aes256Key
+    ensures Result == bkcDigest + aes256Key
   {
-    (mdDigest + aes256Key)
+    (bkcDigest + aes256Key)
   }
 }
